Real triggering on partial invariants. Framing for domains. Bugfix for redefining functions into attributes.

eve/Src/library/base/mml/sequence.bpl
@@ -204,6 +204,15 @@ axiom (forall<T> s: Seq T, i: int, v: T, x: T ::
 axiom (forall<T> s: Seq T, x: T :: { Seq#ToBag(s)[x] } Seq#Has(s, x) <==> 0 < Seq#ToBag(s)[x]);
 axiom (forall<T> s: Seq T, x: T :: { Seq#ToBag(s)[x] } Seq#ToBag(s)[x] == Seq#Occurrences(s, x));
 
+// Sequence converted to map
+function Seq#ToMap<T>(Seq T): Map int T;
+axiom (forall<T> s: Seq T :: { Map#Domain(Seq#ToMap(s)) }
+  Map#Domain(Seq#ToMap(s)) == Seq#Domain(s));
+axiom (forall<T> s: Seq T :: { Map#Card(Seq#ToMap(s)) }
+  Map#Card(Seq#ToMap(s)) == Seq#Length(s));
+axiom (forall<T> s: Seq T, i: int :: { Map#Item(Seq#ToMap(s), i) }
+  1 <= i && i <= Seq#Length(s) ==> Map#Item(Seq#ToMap(s), i) == Seq#Item(s, i));  
+
 // Additional axioms about common things
     
 axiom (forall<T> s, t: Seq T ::
