eve/Src/framework/eiffel2boogie/translation/custom/e2b_custom_ownership_handler.e
@@ -87,13 +87,9 @@ feature -- Basic operations
 					end
 					check_valid_class_inv_tags (l_partial_inv_class, a_translator.context_feature, a_translator.context_line_number, l_tag_filters)
 					translation_pool.add_filtered_invariant_function (a_translator.current_target_type, Void, l_tag_filters, l_partial_inv_class)
-					a_translator.set_last_expression(factory.or_ (
-						factory.function_call ("partial_inv",
-							<< a_translator.entity_mapping.heap, a_translator.current_target >>, types.bool),
-						factory.function_call (
+					a_translator.set_last_expression(factory.function_call (
 							name_translator.boogie_function_for_filtered_invariant (a_translator.current_target_type, Void, l_tag_filters, l_partial_inv_class),
-							<< a_translator.entity_mapping.heap, a_translator.current_target >>, types.bool)
-						))
+							<< a_translator.entity_mapping.heap, a_translator.current_target >>, types.bool))
 				elseif l_name ~ "inv_only" then
 					l_tag_filters := extract_tags (a_parameters)
 					if a_translator.current_target.same_expression (a_translator.entity_mapping.current_expression) then
@@ -103,13 +99,9 @@ feature -- Basic operations
 					end
 					check_valid_class_inv_tags (l_partial_inv_class, a_translator.context_feature, a_translator.context_line_number, l_tag_filters)
 					translation_pool.add_filtered_invariant_function (a_translator.current_target_type, l_tag_filters, Void, l_partial_inv_class)
-					a_translator.set_last_expression(factory.or_ (
-						factory.function_call ("partial_inv",
-							<< a_translator.entity_mapping.heap, a_translator.current_target >>, types.bool),
-						factory.function_call (
-							name_translator.boogie_function_for_filtered_invariant (a_translator.current_target_type, l_tag_filters, Void, l_partial_inv_class),
-							<< a_translator.entity_mapping.heap, a_translator.current_target >>, types.bool)
-						))
+					a_translator.set_last_expression(factory.function_call (
+						name_translator.boogie_function_for_filtered_invariant (a_translator.current_target_type, l_tag_filters, Void, l_partial_inv_class),
+						<< a_translator.entity_mapping.heap, a_translator.current_target >>, types.bool))
 				elseif l_name ~ "inv" then
 					a_translator.process_builtin_routine_call (a_feature, a_parameters, "user_inv")
 				elseif l_name ~ "is_field_writable" then
